verified/smcapi.i.dfy
@@ -1,0 +1,436 @@
+include "smcapi.s.dfy"
+
+//=============================================================================
+// Hoare Specification of Monitor Calls
+//=============================================================================
+function smc_initAddrspace_premium(pageDbIn: PageDb, addrspacePage: PageNr,
+    l1PTPage: PageNr) : (PageDb, int) // PageDbOut, KEV_ERR
+    requires validPageDb(pageDbIn);
+    ensures  validPageDb(smc_initAddrspace_premium(pageDbIn, addrspacePage, l1PTPage).0);
+{
+    initAddrspacePreservesPageDBValidity(pageDbIn, addrspacePage, l1PTPage);
+    smc_initAddrspace(pageDbIn, addrspacePage, l1PTPage)
+}
+
+function smc_initDispatcher_premium(pageDbIn: PageDb, page:PageNr, addrspacePage:PageNr,
+    entrypoint:int) : (PageDb, int) // PageDbOut, KEV_ERR
+    requires validPageDb(pageDbIn);
+    ensures  validPageDb(smc_initDispatcher_premium(pageDbIn, page, addrspacePage, entrypoint).0);
+{
+    smc_initDispatcher(pageDbIn, page, addrspacePage, entrypoint)
+}
+
+function smc_initL2PTable_premium(pageDbIn: PageDb, page: PageNr,
+    addrspacePage: PageNr, l1index: int) : (PageDb, int)
+    requires validPageDb(pageDbIn)
+    ensures validPageDb(smc_initL2PTable_premium(pageDbIn, page, addrspacePage, l1index).0)
+{
+    smc_initL2PTable(pageDbIn, page, addrspacePage, l1index)
+}
+
+function smc_remove_premium(pageDbIn: PageDb, page: PageNr) : (PageDb, int) // PageDbOut, KEV_ERR
+    requires validPageDb(pageDbIn)
+    ensures  validPageDb(smc_remove_premium(pageDbIn, page).0)
+{
+    removePreservesPageDBValidity(pageDbIn, page);
+    smc_remove(pageDbIn, page)
+}
+
+function smc_mapSecure_premium(pageDbIn: PageDb, page: PageNr, addrspacePage: PageNr,
+    mapping: Mapping, physPage: int) : (PageDb, int) // PageDbOut, KEV_ERR
+    requires validPageDb(pageDbIn)
+    ensures  validPageDb(smc_mapSecure_premium(pageDbIn, page, addrspacePage, mapping, physPage).0)
+{
+    mapSecurePreservesPageDBValidity(pageDbIn, page, addrspacePage, mapping, physPage);
+    smc_mapSecure(pageDbIn, page, addrspacePage, mapping, physPage)
+}
+
+function smc_mapInsecure_premium(pageDbIn: PageDb, addrspacePage: PageNr,
+    physPage: int, mapping : Mapping) : (PageDb, int)
+    requires validPageDb(pageDbIn)
+    ensures  validPageDb(smc_mapInsecure_premium(pageDbIn, addrspacePage, physPage, mapping).0)
+{
+    mapInsecurePreservesPageDbValidity(pageDbIn, addrspacePage, physPage, mapping);
+    smc_mapInsecure(pageDbIn, addrspacePage, physPage, mapping)
+}
+
+function smc_finalise_premium(pageDbIn: PageDb, addrspacePage: PageNr) : (PageDb, int)
+    requires validPageDb(pageDbIn)
+    ensures  validPageDb(smc_finalise_premium(pageDbIn, addrspacePage).0)
+{
+    finalisePreservesPageDbValidity(pageDbIn, addrspacePage);
+    smc_finalise(pageDbIn, addrspacePage)
+}
+
+function smc_enter_premium(pageDbIn: PageDb, dispPage: PageNr, arg1: int, arg2: int, arg3: int)
+    : (PageDb, int)
+    requires validPageDb(pageDbIn) 
+    ensures validPageDb(smc_enter_premium(pageDbIn, dispPage, arg1, arg2, arg3).0)
+{
+    enterPreservesPageDbValidity(pageDbIn, dispPage, arg1, arg2, arg3);
+    smc_enter(pageDbIn, dispPage, arg1, arg2, arg3)
+}
+
+function smc_resume_premium(pageDbIn: PageDb, dispPage: PageNr)
+    : (PageDb, int)
+    requires validPageDb(pageDbIn) 
+    ensures validPageDb(smc_resume_premium(pageDbIn, dispPage).0)
+{
+    resumePreservesPageDbValidity(pageDbIn, dispPage);
+    smc_resume(pageDbIn, dispPage)
+}
+
+function smc_stop_premium(pageDbIn: PageDb, addrspacePage: PageNr)
+    : (PageDb, int)
+    requires validPageDb(pageDbIn)
+    ensures  validPageDb(smc_stop_premium(pageDbIn, addrspacePage).0)
+{
+    stopPreservesPageDbValidity(pageDbIn, addrspacePage);
+    smc_stop(pageDbIn, addrspacePage)
+}
+
+function smchandler_premium(pageDbIn: PageDb, callno: int, arg1: int, arg2: int,
+    arg3: int, arg4: int) : (PageDb, int, int) // pageDbOut, err, val
+    requires validPageDb(pageDbIn)
+    ensures validPageDb(smchandler_premium(pageDbIn, callno, arg1, arg2, arg3, arg4).0)
+{
+    smchandlerPreservesPageDbValidity(pageDbIn, callno, arg1, arg2, arg3, arg4);
+    smchandler(pageDbIn, callno, arg1, arg2, arg3, arg4)
+}
+
+//=============================================================================
+// Properties of Monitor Calls
+//=============================================================================
+
+//-----------------------------------------------------------------------------
+// PageDb Validity Preservation
+//-----------------------------------------------------------------------------
+lemma initAddrspacePreservesPageDBValidity(pageDbIn : PageDb,
+    addrspacePage : PageNr, l1PTPage : PageNr)
+    requires validPageDb(pageDbIn)
+    ensures validPageDb(smc_initAddrspace(pageDbIn, addrspacePage, l1PTPage).0)
+{
+     var pageDbOut := smc_initAddrspace(pageDbIn, addrspacePage, l1PTPage).0;
+     var errOut := smc_initAddrspace(pageDbIn, addrspacePage, l1PTPage).1;
+
+     if( errOut != KEV_ERR_SUCCESS() ) {
+        // The error case is trivial because PageDbOut == PageDbIn
+     } else {
+         // Necessary semi-manual proof of validPageDbEntry(pageDbOut, l1PTPage)
+         // The interesting part of the proof deals with the contents of addrspaceRefs
+         assert forall p :: p != l1PTPage ==> !(p in addrspaceRefs(pageDbOut, addrspacePage));
+	     assert l1PTPage in addrspaceRefs(pageDbOut, addrspacePage);
+         assert addrspaceRefs(pageDbOut, addrspacePage) == {l1PTPage};
+         // only kept for readability
+         assert validPageDbEntry(pageDbOut, l1PTPage);
+
+         forall ( n | validPageNr(n)
+             && pageDbOut[n].PageDbEntryTyped?
+             && n != addrspacePage && n != l1PTPage)
+             ensures validPageDbEntryTyped(pageDbOut, n)
+         {
+             assert pageDbOut[n] == pageDbIn[n];
+             assert addrspaceRefs(pageDbOut, n) == addrspaceRefs(pageDbIn, n);
+         }
+              
+         assert pageDbEntriesValid(pageDbOut);
+         assert validPageDb(pageDbOut);
+    }
+}
+
+
+lemma removePreservesPageDBValidity(pageDbIn: PageDb, page: PageNr)
+    requires validPageDb(pageDbIn)
+    ensures  validPageDb(smc_remove(pageDbIn, page).0)
+{
+
+    var pageDbOut := smc_remove(pageDbIn, page).0;
+    var errOut := smc_remove(pageDbIn, page).1;
+
+    if ( errOut != KEV_ERR_SUCCESS() ){
+       // trivial
+    } else if( pageDbIn[page].PageDbEntryFree?) {
+        // trivial
+    } else {
+
+        var entry := pageDbIn[page].entry;
+        var addrspacePage := pageDbIn[page].addrspace;
+
+        forall () ensures validPageDbEntry(pageDbOut, addrspacePage);
+        {
+            if(entry.Addrspace?){
+            } else {
+                var addrspace := pageDbOut[addrspacePage].entry;
+
+                var oldRefs := addrspaceRefs(pageDbIn, addrspacePage);
+                assert addrspaceRefs(pageDbOut, addrspacePage) == oldRefs - {page};
+                assert addrspace.refcount == |addrspaceRefs(pageDbOut, addrspacePage)|;
+                
+                //assert validAddrspace(pageDbOut, addrspace);
+                assert validAddrspacePage(pageDbOut, addrspacePage);
+            }
+        }
+
+        assert validPageDbEntry(pageDbOut, page);
+
+        forall ( n | validPageNr(n) && n != addrspacePage && n != page )
+            ensures validPageDbEntry(pageDbOut, n)
+        {
+            if(pageDbOut[n].PageDbEntryFree?) {
+                // trivial
+            } else {
+                var e := pageDbOut[n].entry;
+                var d := pageDbOut;
+                var a := pageDbOut[n].addrspace;
+
+                assert pageDbOut[n] == pageDbIn[n];
+
+                
+                forall () ensures pageDbEntryOk(d, n){
+                  
+                    // This is a proof that the addrspace of n is still an addrspace
+                    //
+                    // The only interesting case is when the page that was
+                    // removed is the addrspace of n (i.e. a == page). This
+                    // case causes an error because a must have been valid in
+                    // pageDbIn and therefore n has a reference to it.
+                    forall() ensures a in d && d[a].PageDbEntryTyped?
+                        && d[a].entry.Addrspace?;
+                    {
+                        assert a == page ==> n in addrspaceRefs(pageDbIn, a);
+                        assert a == page ==> pageDbIn[a].entry.refcount > 0;
+                        assert a != page;
+                    }
+
+                    if( a == addrspacePage ) {
+                        var oldRefs := addrspaceRefs(pageDbIn, addrspacePage);
+                        assert addrspaceRefs(pageDbOut, addrspacePage) == oldRefs - {page};
+                        assert pageDbOut[a].entry.refcount == |addrspaceRefs(pageDbOut, addrspacePage)|;
+                    } else {
+                        assert pageDbOut[a].entry.refcount == pageDbIn[a].entry.refcount;
+                        assert addrspaceRefs(pageDbIn, a) == addrspaceRefs(pageDbOut, a);
+                    }
+
+                }
+
+            }
+        }
+
+        assert pageDbEntriesValid(pageDbOut);
+        assert validPageDb(pageDbOut);
+    }
+}
+
+lemma mapSecurePreservesPageDBValidity(pageDbIn: PageDb, page: PageNr, addrspacePage: PageNr,
+    mapping: Mapping, physPage: int)
+    requires validPageDb(pageDbIn)
+    ensures  validPageDb(smc_mapSecure(pageDbIn, page, addrspacePage,
+        mapping, physPage).0)
+{
+    var pageDbOut := smc_mapSecure(
+        pageDbIn, page, addrspacePage, mapping, physPage).0;
+    var err := smc_mapSecure(
+        pageDbIn, page, addrspacePage, mapping, physPage).1;
+
+    if( err != KEV_ERR_SUCCESS() ){
+    } else {
+        assert validPageDbEntryTyped(pageDbOut, page);
+        
+        var pageDbA := allocatePage(pageDbIn, page,
+            addrspacePage, DataPage).0;
+       
+        forall() ensures validPageDbEntryTyped(pageDbOut, addrspacePage){
+            var a := addrspacePage;
+            assert pageDbOut[a].entry.refcount == pageDbA[a].entry.refcount;
+            assert addrspaceRefs(pageDbOut, a) == addrspaceRefs(pageDbA, a);
+        }
+
+        forall( n | validPageNr(n)
+            && pageDbOut[n].PageDbEntryTyped?
+            && n != page && n != addrspacePage)
+            ensures validPageDbEntryTyped(pageDbOut, n);
+        {
+            if( pageDbOut[n].entry.Addrspace? ){
+                assert pageDbOut[n].entry.refcount == pageDbA[n].entry.refcount;
+                assert addrspaceRefs(pageDbOut, n) == addrspaceRefs(pageDbA, n);
+            } else {
+                // trivial
+            }
+        }
+    }
+
+}
+
+lemma mapInsecurePreservesPageDbValidity(pageDbIn: PageDb, addrspacePage: PageNr,
+    physPage: int, mapping : Mapping)
+    requires validPageDb(pageDbIn)
+    ensures  validPageDb(smc_mapInsecure(pageDbIn, addrspacePage, physPage, mapping).0)
+{
+    var pageDbOut := smc_mapInsecure(
+        pageDbIn, addrspacePage, physPage, mapping).0;
+    var err := smc_mapInsecure(
+        pageDbIn, addrspacePage, physPage, mapping).1;
+
+    if( err != KEV_ERR_SUCCESS() ){
+    } else {        
+        forall() ensures validPageDbEntryTyped(pageDbOut, addrspacePage){
+            var a := addrspacePage;
+            assert pageDbOut[a].entry.refcount == pageDbIn[a].entry.refcount;
+            assert addrspaceRefs(pageDbOut, a) == addrspaceRefs(pageDbIn, a);
+        }
+
+        forall( n | validPageNr(n)
+            && pageDbOut[n].PageDbEntryTyped?
+            && n != addrspacePage)
+            ensures validPageDbEntryTyped(pageDbOut, n);
+        {
+            if( pageDbOut[n].entry.Addrspace? ){
+                assert pageDbOut[n].entry.refcount == pageDbIn[n].entry.refcount;
+                assert addrspaceRefs(pageDbOut, n) == addrspaceRefs(pageDbIn, n);
+            } else {
+                // trivial
+            }
+        }
+    }
+}
+
+lemma finalisePreservesPageDbValidity(pageDbIn: PageDb, addrspacePage: PageNr)
+    requires validPageDb(pageDbIn)
+    ensures  validPageDb(smc_finalise(pageDbIn, addrspacePage).0)
+{
+    var pageDbOut := smc_finalise(pageDbIn, addrspacePage).0;
+    var err := smc_finalise(pageDbIn, addrspacePage).1;
+
+    if( err != KEV_ERR_SUCCESS() ){
+    } else {
+        var a := addrspacePage;
+        assert pageDbOut[a].entry.refcount == pageDbIn[a].entry.refcount;
+        assert addrspaceRefs(pageDbOut, a) == addrspaceRefs(pageDbIn, a);
+
+        forall ( n | validPageNr(n) 
+            && pageDbOut[n].PageDbEntryTyped?
+            && n != a )
+            ensures validPageDbEntry(pageDbOut, n)
+        {
+            if( pageDbOut[n].entry.Addrspace? ){
+                assert pageDbOut[n].entry.refcount == pageDbIn[n].entry.refcount;
+                assert addrspaceRefs(pageDbOut, n) == addrspaceRefs(pageDbIn, n);
+            } else {
+            }
+
+        }
+    }
+}
+
+lemma enterPreservesPageDbValidity(pageDbIn: PageDb, dispPage: PageNr,
+    arg1: int, arg2: int, arg3: int)
+    requires validPageDb(pageDbIn) 
+    ensures validPageDb(smc_enter(pageDbIn, dispPage, arg1, arg2, arg3).0)
+{
+    var pageDbOut := smc_enter(pageDbIn, dispPage, arg1, arg2, arg3).0;
+    var err := smc_enter(pageDbIn, dispPage, arg1, arg2, arg3).1;
+
+    if( err != KEV_ERR_SUCCESS() ){
+    } else {
+        var a := pageDbOut[dispPage].addrspace;
+        assert pageDbOut[a].entry.refcount == pageDbIn[a].entry.refcount;
+        assert addrspaceRefs(pageDbOut, a) == addrspaceRefs(pageDbIn, a);
+
+        forall ( n | validPageNr(n) 
+            && pageDbOut[n].PageDbEntryTyped?
+            && n != a )
+            ensures validPageDbEntry(pageDbOut, n)
+        {
+            if( pageDbOut[n].entry.Addrspace? ){
+                assert pageDbOut[n].entry.refcount == pageDbIn[n].entry.refcount;
+                assert addrspaceRefs(pageDbOut, n) == addrspaceRefs(pageDbIn, n);
+            } else {
+            }
+
+        }
+    }
+}
+
+lemma resumePreservesPageDbValidity(pageDbIn: PageDb, dispPage: PageNr)
+    requires validPageDb(pageDbIn) 
+    ensures validPageDb(smc_resume(pageDbIn, dispPage).0)
+{
+    var pageDbOut := smc_resume(pageDbIn, dispPage).0;
+    var err := smc_resume(pageDbIn, dispPage).1;
+
+    if( err != KEV_ERR_SUCCESS() ){
+    } else {
+        var a := pageDbOut[dispPage].addrspace;
+        assert pageDbOut[a].entry.refcount == pageDbIn[a].entry.refcount;
+        assert addrspaceRefs(pageDbOut, a) == addrspaceRefs(pageDbIn, a);
+
+        forall ( n | validPageNr(n) 
+            && pageDbOut[n].PageDbEntryTyped?
+            && n != a )
+            ensures validPageDbEntry(pageDbOut, n)
+        {
+            if( pageDbOut[n].entry.Addrspace? ){
+                assert pageDbOut[n].entry.refcount == pageDbIn[n].entry.refcount;
+                assert addrspaceRefs(pageDbOut, n) == addrspaceRefs(pageDbIn, n);
+            } else {
+            }
+
+        }
+
+    }
+}
+
+lemma stopPreservesPageDbValidity(pageDbIn: PageDb, addrspacePage: PageNr)
+    requires validPageDb(pageDbIn)
+    ensures  validPageDb(smc_stop(pageDbIn, addrspacePage).0)
+{
+    var pageDbOut := smc_stop(pageDbIn, addrspacePage).0;
+    var err := smc_stop(pageDbIn, addrspacePage).1;
+
+    if( err != KEV_ERR_SUCCESS() ){
+    } else {
+        var a := addrspacePage;
+        assert pageDbOut[a].entry.refcount == pageDbIn[a].entry.refcount;
+        assert addrspaceRefs(pageDbOut, a) == addrspaceRefs(pageDbIn, a);
+
+        forall ( n | validPageNr(n) 
+            && pageDbOut[n].PageDbEntryTyped?
+            && n != a )
+            ensures validPageDbEntry(pageDbOut, n)
+        {
+            if( pageDbOut[n].entry.Addrspace? ){
+                assert pageDbOut[n].entry.refcount == pageDbIn[n].entry.refcount;
+                assert addrspaceRefs(pageDbOut, n) == addrspaceRefs(pageDbIn, n);
+            } else {
+            }
+
+        }
+
+    }
+}
+
+lemma smchandlerPreservesPageDbValidity(pageDbIn: PageDb, callno: int, arg1: int,
+    arg2: int, arg3: int, arg4: int)
+    requires validPageDb(pageDbIn)
+    ensures validPageDb(smchandler(pageDbIn, callno, arg1, arg2, arg3, arg4).0)
+{
+    if (callno == KEV_SMC_INIT_ADDRSPACE()) {
+        initAddrspacePreservesPageDBValidity(pageDbIn, arg1, arg2);
+    } else if(callno == KEV_SMC_INIT_DISPATCHER()) {
+    } else if(callno == KEV_SMC_INIT_L2PTABLE()) {
+    } else if(callno == KEV_SMC_MAP_SECURE()) {
+        mapSecurePreservesPageDBValidity(pageDbIn, arg1, arg2, intToMapping(arg3), arg4);
+    } else if(callno == KEV_SMC_MAP_INSECURE()) {
+        mapInsecurePreservesPageDbValidity(pageDbIn, arg1, arg2, intToMapping(arg3));
+    } else if(callno == KEV_SMC_REMOVE()) {
+        removePreservesPageDBValidity(pageDbIn, arg1);
+    } else if(callno == KEV_SMC_FINALISE()) {
+        finalisePreservesPageDbValidity(pageDbIn, arg1);
+    } else if(callno == KEV_SMC_ENTER()) {
+        enterPreservesPageDbValidity(pageDbIn, arg1, arg2, arg3, arg4);
+    } else if(callno == KEV_SMC_RESUME()) {
+        resumePreservesPageDbValidity(pageDbIn, arg1);
+    } else if(callno == KEV_SMC_STOP()) {
+        stopPreservesPageDbValidity(pageDbIn, arg1);
+    }
+}
