verified/smcapi.s.dfy
@@ -1,0 +1,432 @@
+include "kev_constants.s.dfy"
+include "pagedb.s.dfy"
+
+predicate pageIsFree(d:PageDb, pg:PageNr)
+    requires pg in d;
+    { d[pg].PageDbEntryFree? }
+
+// a points to an address space and it is closed
+predicate validAddrspacePage(d: PageDb, a: PageNr)
+    requires wellFormedPageDb(d)
+{
+    isAddrspace(d, a) && d[a].entry.l1ptnr in d
+}
+
+predicate physPageInvalid( physPage: int )
+{
+    physPage != 0 && !(physPageIsRam(physPage)
+        && !physPageIsSecure(physPage))
+}
+
+predicate physPageIsRam( physPage: int )
+{
+   physPage * KEVLAR_PAGE_SIZE() < SecurePhysBase()
+}
+
+predicate physPageIsSecure( physPage: int )
+{
+    var paddr := physPage * KEVLAR_PAGE_SIZE();
+    SecurePhysBase() <= paddr < SecurePhysBase() +
+        KEVLAR_SECURE_NPAGES() * KEVLAR_PAGE_SIZE()
+}
+
+predicate l1indexInUse(d: PageDb, a: PageNr, l1index: int)
+    requires validPageDb(d)
+    requires isAddrspace(d, a)
+    requires d[a].entry.state != StoppedState
+    requires 0 <= l1index < NR_L1PTES()
+{
+    var l1ptnr := d[a].entry.l1ptnr;
+    var l1 := d[l1ptnr].entry.l1pt;
+    l1[l1index].Just?
+}
+
+//=============================================================================
+// Mapping
+//=============================================================================
+datatype Mapping = Mapping(l1index: PageNr, l2index: PageNr, perm: Perm)
+datatype Perm = Perm(r: bool, w: bool, x: bool)
+
+function {:opaque} intToMapping(arg: int) : Mapping
+{
+    Mapping(1,1,Perm(false,false,false))
+}
+
+function updateL2Pte(pageDbIn: PageDb, a: PageNr, mapping: Mapping, l2e : L2PTE)
+    : PageDb 
+    requires validPageDb(pageDbIn)
+    requires validPageNr(a)
+    requires isAddrspace(pageDbIn, a)
+    requires isValidMappingTarget(pageDbIn, a, mapping) == KEV_ERR_SUCCESS()
+    requires pageDbIn[a].PageDbEntryTyped? && pageDbIn[a].entry.Addrspace?
+    requires pageDbIn[a].entry.state.InitState?
+{
+    var addrspace := pageDbIn[a].entry;
+    var l1 := pageDbIn[addrspace.l1ptnr].entry;
+    var l1pte := fromJust(l1.l1pt[mapping.l1index]);
+    var l2pt := pageDbIn[l1pte].entry.l2pt;
+    validPageDbImpliesClosedRefs(pageDbIn);
+    pageDbIn[ l1pte := PageDbEntryTyped(a, L2PTable(l2pt[mapping.l2index := l2e])) ]
+
+}
+
+function isValidMappingTarget(d: PageDb, a: PageNr, mapping: Mapping)
+    : int // KEV_ERROR
+    requires validPageDb(d)
+    requires validPageNr(a)
+    requires isAddrspace(d, a)
+{
+    var addrspace := d[a].entry;
+    if(!addrspace.state.InitState?) then
+        KEV_ERR_ALREADY_FINAL()
+    else if(!mapping.perm.r) then KEV_ERR_INVALID_MAPPING()
+    else if(!(0 <= mapping.l1index < NR_L1PTES())
+        || !(0 <= mapping.l2index < NR_L2PTES()) ) then
+        KEV_ERR_INVALID_MAPPING()
+    else
+        var l1 := d[addrspace.l1ptnr].entry;
+        var l1pte := l1.l1pt[mapping.l1index];
+        if(l1pte.Nothing?) then KEV_ERR_INVALID_MAPPING()
+        else KEV_ERR_SUCCESS()
+}
+
+//============================================================================
+// Behavioral Specification of Monitor Calls
+//=============================================================================
+function smc_query() : int { KEV_MAGIC() }
+
+function smc_getPhysPages() : int { KEVLAR_SECURE_NPAGES() }
+
+function smc_initAddrspace(pageDbIn: PageDb, addrspacePage: PageNr, l1PTPage: PageNr)
+    : (PageDb, int) // PageDbOut, KEV_ERR
+    requires validPageDb(pageDbIn);
+{
+    var g := pageDbIn;
+    if(!validPageNr(addrspacePage) || !validPageNr(l1PTPage) ||
+        addrspacePage == l1PTPage) then
+        (pageDbIn, KEV_ERR_INVALID_PAGENO())
+    else if(l1PTPage % 4 != 0) then
+        (pageDbIn, KEV_ERR_INVALID_PAGENO())
+    else if( !g[addrspacePage].PageDbEntryFree? || !g[l1PTPage].PageDbEntryFree? ) then
+        (pageDbIn, KEV_ERR_PAGEINUSE())
+    else
+        var addrspace := Addrspace(l1PTPage, 1, InitState);
+        var l1PT := L1PTable(SeqRepeat(NR_L1PTES(),Nothing));
+        var pageDbOut := 
+            (pageDbIn[addrspacePage := PageDbEntryTyped(addrspacePage, addrspace)])[
+                l1PTPage := PageDbEntryTyped(addrspacePage, l1PT)];
+        (pageDbOut, KEV_ERR_SUCCESS())
+}
+
+function smc_initDispatcher(pageDbIn: PageDb, page:PageNr, addrspacePage:PageNr,
+    entrypoint:int)
+    : (PageDb, int) // PageDbOut, KEV_ERR
+    requires validPageDb(pageDbIn);
+{
+   var n := page;
+   var d := pageDbIn;
+   if(!isAddrspace(pageDbIn, addrspacePage)) then
+       (pageDbIn, KEV_ERR_INVALID_ADDRSPACE())
+   else
+       allocatePage(pageDbIn, page, addrspacePage, Dispatcher(entrypoint, false))
+}
+
+
+function smc_initL2PTable(pageDbIn: PageDb, page: PageNr,
+    addrspacePage: PageNr, l1index: int) : (PageDb, int)
+    requires validPageDb(pageDbIn)
+{
+    if(!(0<= l1index < NR_L1PTES())) then (pageDbIn, KEV_ERR_INVALID_MAPPING())
+    else if(!isAddrspace(pageDbIn, addrspacePage)) then
+        (pageDbIn, KEV_ERR_INVALID_ADDRSPACE())
+
+    // This gets caught later in allocatePage, but putting the check
+    // here means that the addrspace's state will not be stopped for the
+    // l1indexInUse check. The l1indexInUse check assumes that the l1ptnr
+    // is actually an l1pt table, which is true as long as the addrspace
+    // is not stopped.
+    else if(pageDbIn[addrspacePage].entry.state != InitState) then
+        (pageDbIn, KEV_ERR_ALREADY_FINAL())
+    else if(l1indexInUse(pageDbIn, addrspacePage, l1index)) then
+        (pageDbIn, KEV_ERR_ADDRINUSE())
+    else 
+        var l2pt := L2PTable(SeqRepeat(NR_L2PTES(), NoMapping));
+        allocatePage(pageDbIn, page, addrspacePage, l2pt)
+}
+
+// This is not literally an SMC handler. Move elsewhere in file???
+function allocatePage_inner(pageDbIn: PageDb, securePage: PageNr,
+    addrspacePage:PageNr, entry:PageDbEntryTyped)
+    : (PageDb, int) // PageDbOut, KEV_ERR
+    requires validPageDb(pageDbIn)
+    requires validAddrspacePage(pageDbIn, addrspacePage)
+    requires closedRefsPageDbEntry(entry)
+    requires !entry.L1PTable?
+    requires !entry.Addrspace?
+    requires entry.L2PTable? ==>
+        entry.l2pt == SeqRepeat(NR_L2PTES(), NoMapping)
+{
+    var addrspace := pageDbIn[addrspacePage].entry;
+    if(!validPageNr(securePage)) then (pageDbIn, KEV_ERR_INVALID_PAGENO())
+    else if(!pageIsFree(pageDbIn, securePage)) then (pageDbIn, KEV_ERR_PAGEINUSE())
+    else if(addrspace.state != InitState) then
+        (pageDbIn,KEV_ERR_ALREADY_FINAL())
+    // TODO ?? Model page clearing for non-data pages?
+    else
+        var updatedAddrspace := match addrspace
+            case Addrspace(l1, ref, state) => Addrspace(l1, ref + 1, state);
+        var pageDbOut := (pageDbIn[
+            securePage := PageDbEntryTyped(addrspacePage, entry)])[
+            addrspacePage := PageDbEntryTyped(addrspacePage, updatedAddrspace)];
+        (pageDbOut, KEV_ERR_SUCCESS())
+}
+
+// TODO move this elsewhere since it is not a monitor call
+function allocatePage(pageDbIn: PageDb, securePage: PageNr,
+    addrspacePage:PageNr, entry:PageDbEntryTyped )
+    : (PageDb, int) // PageDbOut, KEV_ERR
+    requires validPageDb(pageDbIn)
+    requires validAddrspacePage(pageDbIn, addrspacePage)
+    requires closedRefsPageDbEntry(entry)
+    requires !entry.L1PTable?
+    requires !entry.Addrspace?
+    requires entry.L2PTable? ==>
+        entry.l2pt == SeqRepeat(NR_L2PTES(), NoMapping)
+    ensures  validPageDb(allocatePage(pageDbIn, securePage, addrspacePage, entry).0);
+{
+    allocatePagePreservesPageDBValidity(pageDbIn, securePage, addrspacePage, entry);
+    allocatePage_inner(pageDbIn, securePage, addrspacePage, entry)
+}
+
+function smc_remove(pageDbIn: PageDb, page: PageNr)
+    : (PageDb, int) // PageDbOut, KEV_ERR
+    requires validPageDb(pageDbIn)
+{
+    if(!validPageNr(page)) then
+        (pageDbIn, KEV_ERR_INVALID_PAGENO())
+    else if(pageDbIn[page].PageDbEntryFree?) then
+        (pageDbIn, KEV_ERR_SUCCESS())
+    else 
+        var e := pageDbIn[page].entry;
+        var addrspacePage := pageDbIn[page].addrspace;
+        var addrspace := pageDbIn[addrspacePage].entry;
+        if( e.Addrspace? ) then
+           if(e.refcount !=0) then (pageDbIn, KEV_ERR_PAGEINUSE())
+           else (pageDbIn[page := PageDbEntryFree], KEV_ERR_SUCCESS())
+        else 
+            if( !addrspace.state.StoppedState?) then
+                (pageDbIn, KEV_ERR_NOT_STOPPED())
+            else 
+                assert page in addrspaceRefs(pageDbIn, addrspacePage);
+                var updatedAddrspace := match addrspace
+                    case Addrspace(l1, ref, state) => Addrspace(l1, ref - 1, state);
+                var pageDbOut := (pageDbIn[page := PageDbEntryFree])[
+                    addrspacePage := PageDbEntryTyped(addrspacePage, updatedAddrspace)];
+                (pageDbOut, KEV_ERR_SUCCESS())
+}
+
+function smc_mapSecure(pageDbIn: PageDb, page: PageNr, addrspacePage: PageNr,
+    mapping: Mapping, physPage: int) : (PageDb, int) // PageDbOut, KEV_ERR
+    requires validPageDb(pageDbIn)
+{
+    if(!isAddrspace(pageDbIn, addrspacePage)) then
+        (pageDbIn, KEV_ERR_INVALID_ADDRSPACE())
+    else 
+        var err := isValidMappingTarget(pageDbIn, addrspacePage, mapping);
+        if( err != KEV_ERR_SUCCESS() ) then (pageDbIn, err)
+        else 
+            // I'm not actually sure if this makes sense. I don't know
+            // that physPage is actually modeling a physical page here...
+            // address translation isn't modeled here at all.
+            if( physPageInvalid(physPage) ) then
+                (pageDbIn, KEV_ERR_INVALID_PAGENO())
+            else
+                var ap_ret := allocatePage(pageDbIn, page,
+                    addrspacePage, DataPage);
+                var pageDbA := ap_ret.0;
+                var errA := ap_ret.1;
+                if(errA != KEV_ERR_SUCCESS()) then (pageDbIn, errA)
+                else
+                    var l2pte := SecureMapping(page, mapping.perm.w, mapping.perm.x);
+                    var pageDbOut := updateL2Pte(pageDbA, addrspacePage, mapping, l2pte);
+                    (pageDbOut, KEV_ERR_SUCCESS())
+}
+
+function smc_mapInsecure(pageDbIn: PageDb, addrspacePage: PageNr,
+    physPage: int, mapping : Mapping) : (PageDb, int)
+    requires validPageDb(pageDbIn)
+{
+    if(!isAddrspace(pageDbIn, addrspacePage)) then
+        (pageDbIn, KEV_ERR_INVALID_ADDRSPACE())
+    else
+        var err := isValidMappingTarget(pageDbIn, addrspacePage, mapping);
+        if( err != KEV_ERR_SUCCESS() ) then (pageDbIn, err)
+        else if( physPageIsSecure(physPage) ) then
+            (pageDbIn, KEV_ERR_INVALID_PAGENO())
+        else
+            var l2pte := InsecureMapping( physPage );
+            var pageDbOut := updateL2Pte(pageDbIn, addrspacePage, mapping, l2pte);
+            (pageDbOut, KEV_ERR_SUCCESS())
+}
+
+function smc_finalise(pageDbIn: PageDb, addrspacePage: PageNr) : (PageDb, int)
+    requires validPageDb(pageDbIn)
+{
+    if(!isAddrspace(pageDbIn, addrspacePage)) then
+        (pageDbIn, KEV_ERR_INVALID_ADDRSPACE())
+    else if(pageDbIn[addrspacePage].entry.state != InitState) then
+        (pageDbIn, KEV_ERR_ALREADY_FINAL())
+    else
+        var addrspace := pageDbIn[addrspacePage].entry;
+        var updatedAddrspace := match addrspace
+            case Addrspace(l1, ref, state) => Addrspace(l1, ref, FinalState);
+        var pageDbOut := pageDbIn[
+            addrspacePage := PageDbEntryTyped(addrspacePage, updatedAddrspace)];
+        (pageDbOut, KEV_ERR_SUCCESS())
+}
+
+function smc_enter(pageDbIn: PageDb, dispPage: PageNr, arg1: int, arg2: int, arg3: int)
+    : (PageDb, int)
+    requires validPageDb(pageDbIn)
+{
+    var d := pageDbIn; var p := dispPage;
+    if(!(validPageNr(p) && d[p].PageDbEntryTyped? && d[p].entry.Dispatcher?)) then
+        (pageDbIn, KEV_ERR_INVALID_PAGENO())
+    else if(var a := d[p].addrspace; d[a].entry.state != FinalState) then
+        (pageDbIn, KEV_ERR_NOT_FINAL())
+    else if(d[p].entry.entered) then
+        (pageDbIn, KEV_ERR_ALREADY_ENTERED())
+    else
+        // A model of registers is needed to model more.
+        // For now all this does is change the dispatcher.
+        var a := d[p].addrspace;
+        var pageDbOut := match d[p].entry 
+                case Dispatcher(entrypoint, entered) => 
+                    d[p := PageDbEntryTyped(a,Dispatcher(entrypoint,true))];
+        (pageDbOut, KEV_ERR_SUCCESS())
+}
+
+function smc_resume(pageDbIn: PageDb, dispPage: PageNr)
+    : (PageDb, int)
+    requires validPageDb(pageDbIn)
+{
+    var d := pageDbIn; var p := dispPage;
+    if(!(validPageNr(p) && d[p].PageDbEntryTyped? && d[p].entry.Dispatcher?)) then
+        (pageDbIn, KEV_ERR_INVALID_PAGENO())
+    else if(var a := d[p].addrspace; d[a].entry.state != FinalState) then
+        (pageDbIn, KEV_ERR_NOT_FINAL())
+    else if(!d[p].entry.entered) then
+        (pageDbIn, KEV_ERR_ALREADY_ENTERED())
+    else
+        // A model of registers is needed to model more.
+        // For now all this does is change the dispatcher.
+        var a := d[p].addrspace;
+        var pageDbOut := match d[p].entry 
+                case Dispatcher(entrypoint, entered) => 
+                    d[p := PageDbEntryTyped(a,Dispatcher(entrypoint,false))];
+        (pageDbOut, KEV_ERR_SUCCESS())
+}
+
+function smc_stop(pageDbIn: PageDb, addrspacePage: PageNr)
+    : (PageDb, int)
+    requires validPageDb(pageDbIn)
+{
+    if(!isAddrspace(pageDbIn, addrspacePage)) then
+        (pageDbIn, KEV_ERR_INVALID_ADDRSPACE())
+    // else if(pageDbIn[addrspacePage].entry.state == InitState) then
+    //     (pageDbIn, KEV_ERR_ALREADY_FINAL())
+    else
+        var addrspace := pageDbIn[addrspacePage].entry;
+        var updatedAddrspace := match addrspace
+            case Addrspace(l1, ref, state) => Addrspace(l1, ref, StoppedState);
+        var pageDbOut := pageDbIn[
+            addrspacePage := PageDbEntryTyped(addrspacePage, updatedAddrspace)];
+        (pageDbOut, KEV_ERR_SUCCESS())
+}
+
+//=============================================================================
+// Behavioral Specification of SMC Handler
+//=============================================================================
+function smchandler(pageDbIn: PageDb, callno: int, arg1: int, arg2: int,
+    arg3: int, arg4: int) : (PageDb, int, int) // pageDbOut, err, val
+    requires validPageDb(pageDbIn)
+{
+    if(callno == KEV_SMC_QUERY()) then (pageDbIn, KEV_MAGIC(), 0)
+    else if(callno == KEV_SMC_GETPHYSPAGES()) then
+        (pageDbIn, KEV_ERR_SUCCESS(), KEVLAR_SECURE_NPAGES())
+    else if(callno == KEV_SMC_INIT_ADDRSPACE()) then
+        var ret := smc_initAddrspace(pageDbIn, arg1, arg2);
+        (ret.0, ret.1, 0)
+    else if(callno == KEV_SMC_INIT_DISPATCHER()) then
+        var ret := smc_initDispatcher(pageDbIn, arg1, arg2, arg3);
+        (ret.0, ret.1, 0)
+    else if(callno == KEV_SMC_INIT_L2PTABLE()) then
+        var ret := smc_initL2PTable(pageDbIn, arg1, arg2, arg3);
+        (ret.0, ret.1, 0)
+    else if(callno == KEV_SMC_MAP_SECURE()) then
+        var ret := smc_mapSecure(pageDbIn, arg1, arg2, intToMapping(arg3), arg4);
+        (ret.0, ret.1, 0)
+    else if(callno == KEV_SMC_MAP_INSECURE()) then
+        var ret := smc_mapInsecure(pageDbIn, arg1, arg2, intToMapping(arg3));
+        (ret.0, ret.1, 0)
+    else if(callno == KEV_SMC_REMOVE()) then
+        var ret := smc_remove(pageDbIn, arg1);
+        (ret.0, ret.1, 0)
+    else if(callno == KEV_SMC_FINALISE()) then
+        var ret := smc_finalise(pageDbIn, arg1);
+        (ret.0, ret.1, 0)
+    else if(callno == KEV_SMC_ENTER()) then
+        var ret := smc_enter(pageDbIn, arg1, arg2, arg3, arg4);
+        (ret.0, ret.1, 0)
+    else if(callno == KEV_SMC_RESUME()) then
+        var ret := smc_resume(pageDbIn, arg1);
+        (ret.0, ret.1, 0)
+    else if(callno == KEV_SMC_STOP()) then
+        var ret := smc_stop(pageDbIn, arg1);
+        (ret.0, ret.1, 0)
+    else (pageDbIn, KEV_ERR_INVALID(), 0)
+}
+
+
+// lemma for allocatePage; FIXME: not trusted, should not be in a .s.dfy file
+lemma allocatePagePreservesPageDBValidity(pageDbIn: PageDb,
+    securePage: PageNr, addrspacePage: PageNr, entry: PageDbEntryTyped)
+    requires validPageDb(pageDbIn)
+    requires validAddrspacePage(pageDbIn, addrspacePage)
+    requires closedRefsPageDbEntry(entry)
+    requires !entry.Addrspace?
+    requires !entry.L1PTable?
+    requires entry.L2PTable? ==>
+        entry.l2pt == SeqRepeat(NR_L2PTES(), NoMapping)
+    ensures  validPageDb(allocatePage_inner(
+        pageDbIn, securePage, addrspacePage, entry).0);
+{
+    var pageDbOut := allocatePage_inner(pageDbIn, securePage,
+        addrspacePage, entry).0;
+    var errOut := allocatePage_inner(pageDbIn, securePage,
+        addrspacePage, entry).1;
+
+    if ( errOut != KEV_ERR_SUCCESS() ){
+        // The error case is trivial because PageDbOut == PageDbIn
+    } else {
+      
+        forall () ensures validPageDbEntry(pageDbOut, addrspacePage);
+        {
+            var oldRefs := addrspaceRefs(pageDbIn, addrspacePage);
+            assert addrspaceRefs(pageDbOut, addrspacePage ) == oldRefs + {securePage};
+            
+            var addrspace := pageDbOut[addrspacePage].entry;
+            assert addrspace.refcount == |addrspaceRefs(pageDbOut, addrspacePage)|;
+            assert validAddrspacePage(pageDbOut, addrspacePage);
+        }
+
+        forall ( n | validPageNr(n) && n != addrspacePage && n != securePage )
+            ensures validPageDbEntry(pageDbOut, n)
+        {
+            assert addrspaceRefs(pageDbOut, n) == addrspaceRefs(pageDbIn, n);
+        }
+
+        assert pageDbEntriesValid(pageDbOut);
+        assert validPageDb(pageDbOut);
+    }
+}
